Add comments to Maps module

Maps/Maps.dfy
@@ -14,6 +14,9 @@ module Maps {
 	  imap x | x in m :: m[x]
 	}
 
+  /**
+   * The size of a map is equal to the size of its domain.
+   */
   lemma lemma_size_is_domain_size<X(!new), Y(!new)>(dom: set<X>,
                                                     m: map<X, Y>)
     requires dom == m.Keys
@@ -29,6 +32,9 @@ module Maps {
     }
   }
 
+  /**
+   * Remove all map items with keys that are elements of a set.
+   */
   function method {:opaque} remove_set<X, Y>(m: map<X, Y>, xs: set<X>): (m': map<X, Y>)
     ensures forall x :: x in m && x !in xs ==> x in m'
     ensures forall x :: x in m' ==> x in m && x !in xs && m'[x] == m[x]
@@ -37,6 +43,9 @@ module Maps {
     map x | x in m && x !in xs :: m[x]
   }
 
+  /**
+   * Remove a map item.
+   */
   function method {:opaque} remove<X(!new), Y(!new)>(m: map<X, Y>, x: X): (m': map<X, Y>)
     requires x in m
     ensures forall i :: i in m && i != x ==> i in m'
@@ -48,26 +57,9 @@ module Maps {
     m'
   }
 
-  lemma lemma_remove_decreases_size<X(!new), Y(!new)>(before: map<X, Y>,
-                                                      after: map<X, Y>,
-                                                      item_removed: X)
-    requires item_removed in before
-    requires after == map s | s in before && s != item_removed :: before[s]
-    ensures |after| < |before|
-  {
-    var domain_before := set s | s in before;
-    var domain_after := set s | s in after;
-
-    lemma_size_is_domain_size(domain_before, before);
-    lemma_size_is_domain_size(domain_after, after);
-
-    if |after| == |before| {
-      assert |domain_before - domain_after| > 0;
-    } else if |after| > |before| {
-      assert |domain_after - domain_before| == 0;
-    }
-  }
-
+  /**
+   * Removing a map item decreases map size by 1.
+   */
   lemma lemma_remove_one<X(!new), Y(!new)>(before: map<X, Y>,
                                            after: map<X, Y>,
                                            item_removed: X)
@@ -84,22 +76,45 @@ module Maps {
     assert domain_after + {item_removed} == domain_before;
   }
 
+  /**
+   * Keep all map items with keys that are elements of a set.
+   */
+  function method {:opaque} restrict<X, Y>(m: map<X, Y>, xs: set<X>): map<X, Y> {
+    map x | x in xs && x in m :: m[x]
+  }
+
+  /**
+   * Returns true if a map contains the key-value pair (x, y).
+   */
   predicate {:opaque} contains<X(!new), Y>(m: map<X, Y>, x: X, y: Y) {
     x in m && m[x] == y
   }
 
+  /**
+   * Returns true if two maps are equal for intersecting keys.
+   */
   predicate {:opaque} equals_on_key<X(!new), Y>(m: map<X, Y>, m': map<X, Y>, x: X) {
     (x !in m && x !in m') || (x in m && x in m' && m[x] == m'[x])
   }
 
+  /**
+   * Returns true if two maps are equal.
+   */
   predicate {:opaque} equals<X(!new), Y>(m: map<X, Y>, m': map<X, Y>) {
     (forall x :: x in m <==> x in m') && (forall x :: x in m ==> m[x] == m'[x])
   }
 
+  /**
+   * Returns true if m.Keys is a subset of m'.Keys.
+   */
   predicate {:opaque} is_subset<X(!new), Y>(m: map<X, Y>, m': map<X, Y>) {
     m.Keys <= m'.Keys && (forall x :: x in m ==> equals_on_key(m, m', x))
   }
 
+  /**
+   * Finds the union of two maps. Does not require disjoint domains; on the 
+   * intersection, values from the first map are chosen.
+   */
   function method {:opaque} union_prefer_first<X, Y>(m: map<X, Y>, m': map<X, Y>): (m'': map<X, Y>)
     ensures m''.Keys == m.Keys + m'.Keys
     ensures forall k :: k in m ==> m''[k] == m[k]
@@ -109,6 +124,10 @@ module Maps {
     map x | x in m.Keys + m'.Keys :: if x in m then m[x] else m'[x]
   }
 
+  /**
+   * Finds the union of two maps. Does not require disjoint domains; on the 
+   * intersection, values from the second map are chosen.
+   */
   function method {:opaque} union_prefer_second<X, Y>(m: map<X, Y>, m': map<X, Y>): (m'': map<X, Y>)
     ensures m''.Keys == m.Keys + m'.Keys
     ensures forall k :: k in m' ==> m''[k] == m'[k]
@@ -118,6 +137,10 @@ module Maps {
     map x | x in m.Keys + m'.Keys :: if x in m' then m'[x] else m[x]
   }
 
+  /**
+   * Finds the union of two maps. Does not require disjoint domains; no
+   * promises on which value is chosen on the intersection.
+   */
   function method {:opaque} union<X, Y>(m: map<X, Y>, m': map<X, Y>): (m'': map<X, Y>)
 		ensures m''.Keys == m.Keys + m'.Keys
 		ensures forall k :: k in m.Keys - m'.Keys ==> m[k] == m''[k]
@@ -128,16 +151,10 @@ module Maps {
 		union_prefer_first(m, m')
 	}
 
-  lemma lemma_is_union<X, Y>(m: map<X, Y>, m': map<X, Y>, m'': map<X, Y>)
-    requires m.Keys !! m'.Keys
-    requires forall x :: x in m ==> x in m'' && m''[x] == m[x]
-    requires forall x :: x in m' ==> x in m'' && m''[x] == m'[x]
-    requires forall x :: x in m'' ==> x in m || x in m'
-    ensures m'' == union(m, m')
-	{
-	}
-
-  function method {:opaque} union_disjoint<X, Y>(m: map<X, Y>, m': map<X, Y>): (m'': map<X, Y>)
+  /**
+   * Finds the union of two maps. Requires disjoint domains.
+   */
+  function method {:opaque} disjoint_union<X, Y>(m: map<X, Y>, m': map<X, Y>): (m'': map<X, Y>)
 		requires m.Keys !! m'.Keys
 		ensures m''.Keys == m.Keys + m'.Keys
 		ensures forall k :: k in m ==> m[k] == m''[k]
@@ -146,16 +163,16 @@ module Maps {
 		map x | x in m.Keys + m'.Keys :: if x in m then m[x] else m'[x]
 	}
 
-  lemma lemma_union_disjoint_cardinality<X, Y>(m: map<X, Y>, m': map<X, Y>)
+  /**
+   * The size of the disjoint union is equal to the sum of the sizes of
+   * individual maps.
+   */
+  lemma lemma_disjoint_union_size<X, Y>(m: map<X, Y>, m': map<X, Y>)
     requires m.Keys !! m'.Keys
-    ensures |union_disjoint(m, m')| == |m| + |m'|
+    ensures |disjoint_union(m, m')| == |m| + |m'|
   {
-    var u := union_disjoint(m, m');
+    var u := disjoint_union(m, m');
     assert |u.Keys| == |m.Keys| + |m'.Keys|;
-  }
-
-  function method {:opaque} restrict<X, Y>(m: map<X, Y>, xs: set<X>): map<X, Y> {
-    map x | x in xs && x in m :: m[x]
   }
 
 }
